Partial implementation of unification

ModularEngine/src/LogicEngine.FStar.Wrapper/translationToFStar.fs
@@ -90,7 +90,7 @@ module TranslationToFStar =
     let rec aux (t : ITerm) =
       match t with
       | Forall(v, t') -> let tl, body = aux t' in (v::tl, body)
-      | _ -> t
+      | _ -> [], t
     in let vars, body = aux term in
     match vars with
     | [] -> new Types.MonoTerm(FStarTermOfITerm body)
