ModularEngine/src/LogicEngine.FStar/unify.fst
@@ -2,14 +2,72 @@ module Unify
 open TypeHeaders
 open Types
 open Subst
+open TranslationFromFStar
+
+val fold_left2: ('a -> 'b -> 'c -> option 'a)
+             -> option 'a -> list 'b -> list 'c -> option 'a
+let rec fold_left2 f oa lb lc =
+  match ((oa, lb), lc) with
+  | ((None, _), _) -> None
+  | ((Some(a), []), []) -> oa
+  | ((Some(a), b::tb), c::tc) -> fold_left2 f (f a b c) tb tc
+  | _ -> failwith "Two lists not the same size in fold_left2"
 
 (* ad hoc implementation of unification
      informally, only variables in u are available for unification. *)
-val unify: s1:substitution
-        -> u:vars 
-        -> xs:vars
-        -> i:term    
+val unify: s1:substitution (* this substitution will eventually be applied to goal *)
+        -> u:vars  (* variables available for unification (in goal) *)
+        -> xs:vars (* variables bound in i as foralls *)
+        -> i:term    (* try to unify goal with i *)
         -> goal:term 
         -> option (s2:substitution{Extends s2 s1} * list term)
+val unify_aux: s1:substitution
+            -> u:vars
+            -> xs:vars
+            -> i:term
+            -> goal:term 
+            -> option (s2:substitution{Extends s2 s1})
+
+let rec unify_aux s1 u xs i goal =
+(* should do a pass of backwards chaining here
+   see unifyAndSimpl in logicEngine.fst *)
+  match i with
+  | Types.Var v1 ->
+    (match goal with
+	| _ when (subst i s1:term) = subst goal s1 -> Some s1
+	| _ when not(contains v1 (freeVars goal)) && contains v1 u ->
+	   if inDomain s1 v1
+	   then unify_aux s1 u xs (subst i s1) goal
+	   else failwith "TODO" (* TODO Some(extendSubst s1 v1 (subst goal s1)) *)
+	| _ -> None)
+  | Types.Const c1 ->
+    (match goal with
+	 | _ when i = subst goal s1 -> Some(s1)
+	 | Types.Var v2 -> unify_aux s1 xs u goal i
+	 | _ -> None)
+  | Types.App(f1, tlist1) ->
+    (match goal with
+	 | Types.Var v2 -> unify_aux s1 xs u goal i
+	 (*| Types.App(f2, tlist2) when (f1 = f2) 
+	                           && (length tlist1 = length tlist2) ->
+         fold_left2 (fun (s:substitution{Extends s s1}) (t1:term) (t2:term) 
+		               -> unify_aux s u xs t1 t2)
+		   (Some(s1)) tlist1 tlist2 *)
+	 | _ -> None)
+  (*| Types.SubstrateQueryTerm t0 ->
+      option_map (fun s2 -> (s2, substList (map (fun x -> Types.Var x) xs) s2))
+        (option_map FStarSubstitutionOfISubstitution
+          (substrateQueryTerm_unifyFrom t0 (ISubstitutionOfFStarSubstitution s1) 
+		                                (ITermOfFStarTerm goal) ) )
+  | Types.SubstrateUpdateTerm t0 ->
+      option_map (fun s2 -> (s2, substList (map (fun x -> Types.Var x) xs) s2))
+        (option_map FStarSubstitutionOfISubstitution
+          (substrateQueryTerm_unifyFrom t0 (ISubstitutionOfFStarSubstitution s1)
+		                                (ITermOfFStarTerm goal) ) )*)
+
+let unify s1 u xs i goal =
+  match unify_aux s1 u xs i goal with
+  | None -> None
+  | Some s2 -> Some(s2, substList (map (fun v -> Var(v)) xs) s2)
 
 
